src/MicroSail/Syntax.v
@@ -27,12 +27,16 @@
 (******************************************************************************)
 
 From Coq Require Import
+     Bool.Bool
      Logic.EqdepFacts
      Logic.FunctionalExtensionality
      Program.Equality
      Program.Tactics
      Strings.String
      ZArith.ZArith.
+
+From Equations Require Import
+     Equations Signature.
 
 From MicroSail Require Export
      Context
@@ -49,6 +53,18 @@ Inductive Bit : Set := bitzero | bitone.
 Inductive teq {I} {F : I -> Type} {i j} (fi : F i) (fj : F j) : Prop :=
 | teq_refl (eqi : i = j) (eqf : eq_rect _ _ fi _ eqi = fj) : teq fi fj.
 Infix "≡" := teq (at level 70, no associativity).
+
+Definition Bit_eqb (b1 : Bit) (b2 : Bit) : bool :=
+  match b1, b2 with
+  | bitzero, bitzero => true
+  | bitone , bitone  => true
+  | _      , _       => false
+  end.
+
+Lemma Bit_eqb_spec (b1 b2 : Bit) : reflect (b1 = b2) (Bit_eqb b1 b2).
+Proof.
+  destruct b1; destruct b2; cbn; constructor; congruence.
+Qed.
 
 (******************************************************************************)
 
@@ -124,6 +140,7 @@ Module Type TypeKit.
   Parameter Inline 𝑬_eq_dec : forall x y : 𝑬, {x=y}+{~x=y}.
   (* Names of enum data constructors. *)
   Parameter Inline 𝑬𝑲 : 𝑬 -> Set.
+  Parameter Inline 𝑬𝑲_eq_dec : forall (e : 𝑬) (x y : 𝑬𝑲 e), {x=y}+{~x=y}.
   Declare Instance Blastable_𝑬𝑲 : forall E, Blastable (𝑬𝑲 E).
 
   (* Names of union type constructors. *)
@@ -131,8 +148,10 @@ Module Type TypeKit.
   Parameter Inline 𝑼_eq_dec : forall x y : 𝑼, {x=y}+{~x=y}.
   (* Union types. *)
   Parameter Inline 𝑼𝑻  : 𝑼 -> Set.
+  Parameter Inline 𝑼𝑻_eq_dec : forall (u : 𝑼) (x y : 𝑼𝑻 u), {x=y}+{~x=y}.
   (* Names of union data constructors. *)
   Parameter Inline 𝑼𝑲  : 𝑼 -> Set.
+  Parameter Inline 𝑼𝑲_eq_dec : forall (u : 𝑼) (x y : 𝑼𝑲 u), {x=y}+{~x=y}.
   Declare Instance Blastable_𝑼𝑲 : forall U, Blastable (𝑼𝑲 U).
 
   (* Names of record type constructors. *)
@@ -140,6 +159,7 @@ Module Type TypeKit.
   Parameter Inline 𝑹_eq_dec : forall x y : 𝑹, {x=y}+{~x=y}.
   (* Record types. *)
   Parameter Inline 𝑹𝑻  : 𝑹 -> Set.
+  Parameter Inline 𝑹𝑻_eq_dec : forall (r : 𝑹) (x y : 𝑹𝑻 r), {x=y}+{~x=y}.
   (* Names of expression variables. *)
   Parameter Inline 𝑿 : Set. (* input: \MIX *)
   (* For name resolution we rely on decidable equality of expression
@@ -153,9 +173,10 @@ End TypeKit.
 
 Module Types (Export typekit : TypeKit).
 
+  Local Set Transparent Obligations.
   Local Unset Elimination Schemes.
 
-  Inductive Ty : Set :=
+  Inductive Ty : Type :=
   | ty_int
   | ty_bool
   | ty_bit
@@ -170,6 +191,8 @@ Module Types (Export typekit : TypeKit).
   | ty_union (U : 𝑼)
   | ty_record (R : 𝑹)
   .
+
+  Derive NoConfusion for Ty.
 
   Section ty_rect.
     Variable P  : Ty -> Type.
@@ -393,6 +416,76 @@ Module Terms (typekit : TypeKit) (termkit : TermKit typekit).
       | ty_record R => blastable_record R
       end%type.
 
+    (* Ask Coq to generate boolean and decidable equality for list *)
+    Scheme Equality for list.
+    Lemma list_beq_spec :
+      forall (A : Type) (xs ys : list A)
+        (A_eqb : A -> A -> bool) (A_eqb_spec : forall x y, reflect (x = y) (A_eqb x y)) ,
+        reflect (xs = ys) (list_beq A_eqb xs ys).
+    Proof with cbn; try (constructor; congruence).
+      intros.
+      revert ys.
+      induction xs as [|x xs]; intros [|y ys]...
+      - destruct (A_eqb_spec x y); destruct (IHxs ys)...
+    Qed.
+    Scheme Equality for prod.
+    Scheme Equality for sum.
+
+    Equations Lit_eqb σ (l1 l2 : Lit σ) : bool :=
+      Lit_eqb ty_int l1 l2 := Z.eqb l1 l2;
+      Lit_eqb ty_bool  l1 l2 := Bool.eqb l1 l2;
+      Lit_eqb ty_bit  l1 l2 := Bit_eqb l1 l2;
+      Lit_eqb ty_string l1 l2 := String.eqb l1 l2;
+      Lit_eqb (ty_list τ) l1 l2 := list_beq (Lit_eqb τ) l1 l2;
+      Lit_eqb (ty_prod τ1 τ2) l1 l2 := prod_beq (Lit_eqb τ1) (Lit_eqb τ2) l1 l2;
+      Lit_eqb (ty_sum τ1 τ2) l1 l2 := sum_beq (Lit_eqb τ1) (Lit_eqb τ2) l1 l2;
+      Lit_eqb ty_unit _ _ := true;
+      Lit_eqb (ty_enum e) l1 l2 :=
+        match 𝑬𝑲_eq_dec l1 l2 with
+        | left eq_refl => true
+        | right _ => false
+        end;
+      Lit_eqb (ty_tuple σs) l1 l2 := envrec_beq Lit_eqb l1 l2;
+      Lit_eqb (ty_union U) l1 l2 :=
+        match @𝑼𝑻_eq_dec U l1 l2 with
+        | left eq_refl => true
+        | right _ => false
+        end;
+      Lit_eqb (ty_record R) l1 l2 :=
+        match @𝑹𝑻_eq_dec R l1 l2 with
+        | left eq_refl => true
+        | right _ => false
+        end.
+
+    Lemma Lit_eqb_spec (σ : Ty) (x y : Lit σ) : reflect (x = y) (Lit_eqb σ x y).
+    Proof with cbn; try (constructor; congruence).
+      induction σ; simp Lit_eqb; cbn.
+      - apply Z.eqb_spec.
+      - apply Bool.eqb_spec.
+      - apply Bit_eqb_spec.
+      - apply String.eqb_spec.
+      - revert y.
+        induction x as [|x xs]; intros [|y ys]...
+        destruct (IHσ x y); destruct (IHxs ys)...
+      - destruct x as [x1 x2]; destruct y as [y1 y2]; cbn.
+        destruct (IHσ1 x1 y1); destruct (IHσ2 x2 y2)...
+      - destruct x as [x1| x2]; destruct y as [y1|y2]; cbn.
+        + destruct (IHσ1 x1 y1)...
+        + constructor; congruence.
+        + constructor; congruence.
+        + destruct (IHσ2 x2 y2)...
+      - destruct x. destruct y...
+      - destruct (𝑬𝑲_eq_dec x y) as [e | bot ]; try (destruct e)...
+      - induction σs; intros.
+        + destruct x; destruct y...
+        + cbn in *.
+          destruct x as [xs x]; destruct y as [ys y]; destruct X as [pb pσs]; cbn in *.
+          specialize (IHσs pσs).
+          destruct (IHσs xs ys); destruct (pb x y)...
+      - destruct (𝑼𝑻_eq_dec x y) as [e | bot]; try destruct e...
+      - destruct (𝑹𝑻_eq_dec x y) as [e | bot]; try destruct e...
+    Qed.
+
   End Literals.
   Bind Scope lit_scope with Lit.
 
@@ -467,7 +560,7 @@ Module Terms (typekit : TypeKit) (termkit : TermKit typekit).
 
     Fixpoint eval {Γ : Ctx (𝑿 * Ty)} {σ : Ty} (e : Exp Γ σ) (δ : LocalStore Γ) {struct e} : Lit σ :=
       match e in (Exp _ t) return (Lit t) with
-      | exp_var x           => δ ! x
+      | exp_var x           => δ ‼ x
       | exp_lit _ _ l       => l
       | exp_plus e1 e2      => Z.add (eval e1 δ) (eval e2 δ)
       | exp_times e1 e2     => Z.mul (eval e1 δ) (eval e2 δ)
@@ -497,7 +590,7 @@ Module Terms (typekit : TypeKit) (termkit : TermKit typekit).
                                          (fun σs _ => Env' Lit σs)
                                          env_nil
                                          (fun σs _ vs _ e => env_snoc vs _ (eval e δ)) es)
-      | exp_projrec e rf    => 𝑹_unfold (eval e δ) ! rf
+      | exp_projrec e rf    => 𝑹_unfold (eval e δ) ‼ rf
       | exp_builtin f e     => f (eval e δ)
       end.
 
@@ -509,7 +602,7 @@ Module Terms (typekit : TypeKit) (termkit : TermKit typekit).
 
   Section Statements.
 
-    Inductive TuplePat : Ctx Ty -> Ctx (𝑿 * Ty) -> Set :=
+    Inductive TuplePat : Ctx Ty -> Ctx (𝑿 * Ty) -> Type :=
     | tuplepat_nil  : TuplePat ctx_nil ctx_nil
     | tuplepat_snoc
         {σs : Ctx Ty} {Δ : Ctx (𝑿 * Ty)}
@@ -517,7 +610,7 @@ Module Terms (typekit : TypeKit) (termkit : TermKit typekit).
         TuplePat (ctx_snoc σs σ) (ctx_snoc Δ (x , σ)).
     Bind Scope pat_scope with TuplePat.
 
-    Inductive RecordPat : Ctx (𝑹𝑭 * Ty) -> Ctx (𝑿 * Ty) -> Set :=
+    Inductive RecordPat : Ctx (𝑹𝑭 * Ty) -> Ctx (𝑿 * Ty) -> Type :=
     | recordpat_nil  : RecordPat ctx_nil ctx_nil
     | recordpat_snoc
         {rfs : Ctx (𝑹𝑭 * Ty)} {Δ : Ctx (𝑿 * Ty)}
@@ -627,25 +720,25 @@ Module Terms (typekit : TypeKit) (termkit : TermKit typekit).
 
   Module NameResolution.
 
-    Fixpoint ctx_resolve {D : Set} (Γ : Ctx (𝑿 * D)) (x : 𝑿) {struct Γ} : option D :=
+    Fixpoint ctx_resolve {D : Type} (Γ : Ctx (𝑿 * D)) (x : 𝑿) {struct Γ} : option D :=
       match Γ with
       | ctx_nil           => None
       | ctx_snoc Γ (y, d) => if 𝑿_eq_dec x y then Some d else ctx_resolve Γ x
       end.
 
-    Definition IsSome {D : Set} (m : option D) : Set :=
+    Definition IsSome {D : Type} (m : option D) : Type :=
       match m with
         | Some _ => unit
         | None => Empty_set
       end.
 
-    Definition fromSome {D : Set} (m : option D) : IsSome m -> D :=
+    Definition fromSome {D : Type} (m : option D) : IsSome m -> D :=
       match m return IsSome m -> D with
       | Some d => fun _ => d
       | None   => fun p => match p with end
       end.
 
-    Fixpoint mk_inctx {D : Set} (Γ : Ctx (prod 𝑿 D)) (x : 𝑿) {struct Γ} :
+    Fixpoint mk_inctx {D : Type} (Γ : Ctx (prod 𝑿 D)) (x : 𝑿) {struct Γ} :
       let m := ctx_resolve Γ x in forall (p : IsSome m), InCtx (x , fromSome m p) Γ :=
       match Γ with
       | ctx_nil => fun p => match p with end
